src/core/DY.Core.Trace.Invariant.fst
@@ -52,11 +52,57 @@ type state_predicate {|crypto_invariants|} = {
   ;
 }
 
+/// The state update predicate can be used to constrain how a principal's state is allowed
+/// to evolve over time, for instance, requiring that some fields of the state are constant
+/// once set, or that a counter is monotonically increasing.
+/// To update a state (i.e., write to a principal, state_id pair that already had a state
+/// entry on the current trace), the state predicate needs to hold for the new state, but
+/// also the update predicate must hold, relating the old and new states (at the trace/time
+/// where the update is taking place).
+
+noeq
+type state_update_predicate {|crypto_invariants|} = {
+  update_pred: trace -> principal -> state_id -> bytes -> bytes -> prop;
+  // TODO Should this hold? It seems quite natural that if an update
+  // from A to B was allowed, it remains allowed. This works because we
+  // talk about both the start and end of the update, rather than saying
+  // "it is allowed to update from [current value] to B".
+  update_pred_later:
+    tr1:trace -> tr2:trace ->
+    prin:principal -> sess_id:state_id ->
+    b1:bytes -> b2:bytes ->
+    Lemma
+    (requires update_pred tr1 prin sess_id b1 b2)
+    (ensures update_pred tr2 prin sess_id b1 b2)
+  ;
+  // Do we want transitivity?
+  update_pred_trans:
+    tr:trace ->
+    prin:principal -> sess_id:state_id ->
+    b1:bytes -> b2:bytes -> b3:bytes ->
+    Lemma
+    (requires
+      update_pred tr prin sess_id b1 b2 /\
+      update_pred tr prin sess_id b2 b3
+    )
+    (ensures update_pred tr prin sess_id b1 b3)
+  ;
+  // Reflexivity too?
+}
+
+// Transitivity:
+// - Pred transitive for any given trace?
+//   - Would also need a later pred saying that the update pred is stable.
+//   - Do these two hold? Probably easier to use than a single mixed transitivity pred.
+// - Pred transitive as in later pred above?
+//
+
 /// The parameters of the trace invariant.
 
 noeq
 type trace_invariants {|crypto_invariants|} = {
   state_pred: state_predicate;
+  state_update_pred: state_update_predicate;
   event_pred: trace -> principal -> string -> bytes -> prop;
 }
 
@@ -76,6 +122,7 @@ class protocol_invariants = {
 // hence we simulate inheritance like this.
 
 let state_pred {|invs:protocol_invariants|} = invs.trace_invs.state_pred
+let state_update_pred {|invs:protocol_invariants|} = invs.trace_invs.state_update_pred
 let event_pred {|invs:protocol_invariants|} = invs.trace_invs.event_pred
 
 (*** Trace invariant definition ***)
@@ -90,7 +137,21 @@ let trace_entry_invariant #invs tr entry =
     is_publishable tr msg
   | SetState prin sess_id content -> (
     // Stored states satisfy the custom state predicate
-    invs.trace_invs.state_pred.pred tr prin sess_id content
+    invs.trace_invs.state_pred.pred tr prin sess_id content /\
+    (
+      let is_state_for prin sess_id e =
+        match e with
+        | SetState prin' sess_id' content -> prin = prin' && sess_id = sess_id'
+        | _ -> false
+      in
+      let ts_old_opt = trace_search_last tr (is_state_for prin sess_id) in
+      match ts_old_opt with
+      | None -> True
+      | Some ts_old -> (
+        let SetState _ _ content_old = get_entry_at tr ts_old in
+        invs.trace_invs.state_update_pred.update_pred tr prin sess_id content_old content
+      )
+    )
   )
   | Event prin tag content -> (
     // Triggered protocol events satisfy the custom event predicate
@@ -212,6 +273,44 @@ val state_is_knowable_by:
   (ensures is_knowable_by (principal_state_content_label prin sess_id content) tr content)
 let state_is_knowable_by #invs tr prin sess_id content =
   state_pred.pred_knowable tr prin sess_id content
+
+/// If a state was known to be set at two different times, its value at those times
+/// must be related by the update predicate.
+
+val state_was_set_twice_implies_update_pred:
+  {|protocol_invariants|} -> tr:trace ->
+  ts1:timestamp -> ts2:timestamp ->
+  prin:principal -> sess_id:state_id ->
+  content1:bytes -> content2:bytes ->
+  Lemma
+  (requires
+    state_was_set_at tr ts1 prin sess_id content1 /\
+    state_was_set_at tr ts2 prin sess_id content2 /\
+    ts1 < ts2 /\
+    trace_invariant tr
+  )
+  (ensures
+    state_update_pred.update_pred tr prin sess_id content1 content2
+  )
+let rec state_was_set_twice_implies_update_pred tr ts1 ts2 prin sess_id content1 content2 =
+  let is_state_for prin sess_id e =
+    match e with
+    | SetState prin' sess_id' content -> prin = prin' && sess_id = sess_id'
+    | _ -> false
+  in
+  let Some ts' = trace_search_last (prefix tr ts2) (is_state_for prin sess_id) in
+  let SetState _ _ content' = get_entry_at tr ts' in
+
+  entry_at_implies_trace_entry_invariant tr ts2 (SetState prin sess_id content2);
+  state_update_pred.update_pred_later (prefix tr ts2) tr prin sess_id content' content2;
+
+  if ts1 < ts'
+  then (
+    state_was_set_twice_implies_update_pred tr ts1 ts' prin sess_id content1 content';
+    state_update_pred.update_pred_trans tr prin sess_id content1 content' content2;
+    ()
+  )
+  else ()
 
 /// Triggered protocol events satisfy the event predicate.
 
